\section*{Question 1}

Let X be a discrete random variable with pmf given by
\begin{equation*}
    f_X(k) = e^{-\lambda} \frac{\lambda^k}{k!}, \quad k = 0, 1, 2, \ldots
\end{equation*}
Show that its mgf is \(M_X(t) = e^{\lambda(e^t - 1)}\).
Using this calculate \(E[X^2]\).

\subsection*{Solution}

Poisson random variable.

The mgf is defined by \( M_X(t) = \operatorname{E}{e^{tX}} \), where \( \operatorname{E} \) denotes the expectation.
\begin{align*}
    M_X(t)
     & =
    \operatorname{E}{e^{tX}}
    = \sum_{k=0}^{\infty} e^{tk} e^{-\lambda} \frac{\lambda^k}{k!}
    = e^{-\lambda} \sum_{k=0}^{\infty} \frac{{(\lambda e^t)}^k}{k!}
    \\ & =
    e^{-\lambda} e^{\lambda e^t}
    =
    \boxed{
        e^{\lambda(e^t - 1)}
    }
\end{align*}

Differentiating the mgf twice and evaluating at \( t = 0 \) gives the second moment.
\begin{align*}
    M_X''(t)
     & =
    \frac{d^2}{dt^2} e^{\lambda(e^t - 1)}
    =
    \frac{d}{dt} (e^{\lambda(e^t - 1)} \lambda e^t)
    =
    \lambda e^{\lambda(e^t - 1) + t} (\lambda e^t + 1)
    \\ &
    \implies
    E[X^2]
    = M_X''(0)
    = \lambda e^{\lambda(1 - 1) + 0} (\lambda + 1)
    = \boxed{\lambda(\lambda + 1)}
\end{align*}
