\section*{Question 1}
\setcounter{section}{1}
\setcounter{equation}{0}

Let \( X, Y \) be iid geometric random variables with parameter \( p \).
(The geometric pmf is: \( f_{X}(k)=f_{Y}(k)={(1-p)}^{k-1} p, k=1,2, \dots \)).
Let \( Z=X-Y \) and \( W=\min (X, Y) \).
Find the joint mass function of \( Z, W \).
Show that \( Z, W \) are independent.

\subsection*{Solution}

The joint mass function of \( Z, W \) is given by
\begin{equation*}
    f_{ZW}(z, w)
    =
    P[Z=z, W=w]
    =
    P[X-Y=z, \min (X, Y)=w]
\end{equation*}
Now, we can see that
\begin{equation}
    [\min (X, Y)=w]
    =
    [X=w, Y>w] \cup [X>w, Y=w] \cup [X=w, Y=w]
\end{equation}
which are disjoint events.
Thereby, we have
\begin{align*}
    f_{ZW}(z, w)
     & =
    P[X-Y=z, \min (X, Y)=w]
    \\ & =
    P[X-Y=z, X=w, Y>w]
    + P[X-Y=z, X>w, Y=w]
    \\ & \qquad
    + P[X-Y=z, X=w, Y=w]
    \\ & =
    P[X=w, Y=w-z]
    + P[X=w+z, Y=w]
    + P[X=w, Y=w]
    \\ & =
    P[X=w] P[Y=w-z]
    + P[X=w+z] P[Y=w]
    + P[X=w] P[Y=w]
    \\ & =
    f_{X}(w) f_{Y}(w-z)
    + f_{X}(w+z) f_{Y}(w)
    + f_{X}(w) f_{Y}(w)
    \\ & =
    {(1-p)}^{w-1} p {(1-p)}^{w-z-1} p
    + {(1-p)}^{w+z-1} p {(1-p)}^{w-1} p
    \\ & \qquad
    + {(1-p)}^{w-1} p {(1-p)}^{w-1} p
    \\ & =
    {(1-p)}^{2w-1} p^{2} {(1-p)}^{-z}
    + {(1-p)}^{2w-1} p^{2} {(1-p)}^{z}
    + {(1-p)}^{2w-2} p^{2}
    \\ & =
    {(1-p)}^{2w-2} p^{2} \left( {(1-p)}^{-z} + {(1-p)}^{z} + 1 \right)
\end{align*}

Now, we can see that
\begin{align*}
    \implies
    f_{Z}(z)
     & =
    \sum_{w=1}^{\infty} f_{ZW}(z, w)
    \\ & =
    \sum_{w=1}^{\infty} {(1-p)}^{2w-2} p^{2} \left( {(1-p)}^{-z} + {(1-p)}^{z} + 1 \right)
    \\ & =
    p^{2} \left( {(1-p)}^{-z} + {(1-p)}^{z} + 1 \right) \sum_{w=1}^{\infty} {(1-p)}^{2w-2}
    \\ & =
    p^{2} \left( {(1-p)}^{-z} + {(1-p)}^{z} + 1 \right) \sum_{w=0}^{\infty} {(1-p)}^{2w}
    \\ & =
    p^{2} \left( {(1-p)}^{-z} + {(1-p)}^{z} + 1 \right) \frac{1}{{1-(1-p)^{2}}}
    \\ & =
    p^{2} \left( {(1-p)}^{-z} + {(1-p)}^{z} + 1 \right) \frac{1}{2p-p^{2}}
    \\ & =
    \frac{p}{2-p} \left( {(1-p)}^{-z} + {(1-p)}^{z} + 1 \right)
    \\
    \implies
    f_{W}(w)
     & =
    \sum_{z=-\infty}^{\infty} f_{ZW}(z, w)
    \\ & =
    \sum_{z=-\infty}^{\infty} {(1-p)}^{2w-2} p^{2} \left( {(1-p)}^{-z} + {(1-p)}^{z} + 1 \right)
    \\ & =
    p^{2} {(1-p)}^{2w-2} \left( \sum_{z=-\infty}^{\infty} {(1-p)}^{-z} + \sum_{z=-\infty}^{\infty} {(1-p)}^{z} + \sum_{z=-\infty}^{\infty} 1 \right)
    \\ & =
    p^{2} {(1-p)}^{2w-2} \left( \frac{1}{1-(1-p)} + \frac{1}{1-(1-p)} \right)
    \\ & =
    p^{2} {(1-p)}^{2w-2} \left( \frac{1}{p} + \frac{1}{p} \right)
    \\ & =
    2 p {(1-p)}^{2w-2}
\end{align*}

Now, we can see that
\begin{align*}
    f_{Z}(z) f_{W}(w)
     & =
    \frac{p}{2-p} \left( {(1-p)}^{-z} + {(1-p)}^{z} + 1 \right) 2 p {(1-p)}^{2w-2}
    \\ & =
    \frac{2p^{2}}{2-p} {(1-p)}^{2w-2} \left( {(1-p)}^{-z} + {(1-p)}^{z} + 1 \right)
    \\ & =
    \frac{2p^{2}}{2-p} f_{ZW}(z, w)
\end{align*}
