\section*{Question 2}

Let \( X \) be uniform over \( (0,2) \) and let \( Y \) be a discrete random variable taking non-negative integer values.
Suppose \( X, Y \) are independent.
Let \( Z=X+Y \).
Show that \( Z \) is a continuous random variable.

\subsection*{Solution}

We have that \( X \sim U(0,2) \) and \( Y \) is a discrete random variable, taking non-negative integer values.
Since \( X, Y \) are independent, we have that
\begin{equation*}
    f_{XY}(x, y)
    =
    f_{X}(x) f_{Y}(y)
\end{equation*}
where \( f_{X}(x) \) is the probability density function of \( X \) and \( f_{Y}(y) \) is the probability mass function of \( Y \).
Now, we can find the distribution function of \( Z \) as follows
\begin{align*}
    F_{Z}(z)
     & =
    P[Z \leq z]
    =
    P[X+Y \leq z]
    \\ & =
    \sum_{y=0}^{\infty} P[X+Y \leq z \mid Y=y] P[Y=y]
    \\ & =
    \sum_{y=0}^{\infty} P[X \leq z-y] P[Y=y]
\end{align*}

Now, we can see that
\begin{equation*}
    F_{X}(x)
    =
    P[X \leq x]
    =
    \begin{cases}
        0           & x < 0        \\
        \frac{x}{2} & 0 \leq x < 2 \\
        1           & x \geq 2
    \end{cases}
\end{equation*}

Now, for \( z \leq 0 \), we have
\begin{align*}
    F_{Z}(z)
     & =
    \cancel{P[X \leq z]} P[Y = 0]
    +
    \cancel{P[X \leq z-1]} P[Y = 1]
    \\ & \qquad +
    \cancel{P[X \leq z-2]} P[Y = 2]
    +
    \ldots
    \\
    \implies
    F_{Z}(z)
     & =
    0
\end{align*}

Now, for \( z \in [0, 1] \), we have
\begin{align*}
    F_{Z}(z)
     & =
    P[X \leq z] P[Y = 0]
    +
    \cancel{P[X \leq z-1]} P[Y = 1]
    +
    \ldots
    \\ & =
    \frac{z}{2} \cdot P[Y = 0]
\end{align*}

Now, for \( z \in [1, 2] \), we have
\begin{align*}
    F_{Z}(z)
     & =
    P[X \leq z] P[Y = 0]
    +
    P[X \leq z-1] P[Y = 1]
    \\ & \qquad +
    \cancel{P[X \leq z-2]} P[Y = 2]
    +
    \cancel{P[X \leq z-3]} P[Y = 3]
    +
    \ldots
    \\ & =
    \frac{z}{2} \cdot P[Y = 0]
    +
    \frac{z-1}{2} \cdot P[Y = 1]
\end{align*}

Now, for \( z \in [2, 3] \), we have
\begin{align*}
    F_{Z}(z)
     & =
    P[X \leq z] P[Y = 0]
    +
    P[X \leq z-1] P[Y = 1]
    \\ & \qquad +
    P[X \leq z-2] P[Y = 2]
    +
    \cancel{P[X \leq z-3]} P[Y = 3]
    +
    \ldots
    \\ & =
    1 \cdot P[Y = 0]
    +
    \frac{z-1}{2} \cdot P[Y = 1]
    +
    \frac{z-2}{2} \cdot P[Y = 2]
\end{align*}

Now, for \( z \in [3, 4] \), we have
\begin{align*}
    F_{Z}(z)
     & =
    P[X \leq z] P[Y = 0]
    +
    P[X \leq z-1] P[Y = 1]
    \\ & \qquad +
    P[X \leq z-2] P[Y = 2]
    +
    P[X \leq z-3] P[Y = 3]
    +
    \ldots
    \\ & =
    1 \cdot P[Y = 0]
    +
    1 \cdot P[Y = 1]
    +
    \frac{z-2}{2} \cdot P[Y = 2]
    +
    \frac{z-3}{2} \cdot P[Y = 3]
\end{align*}
