\section*{Question 5}
\setcounter{section}{5}
\setcounter{equation}{0}

Suppose \( \Lambda \) is a continuous random variable with density \( f_{\Lambda}(\lambda)=e^{-\lambda}, 0< \) \( \lambda<\infty \).
Let \( X \) be a discrete random variable whose conditional mass function, conditioned on \( \Lambda \), is given by
\[
    f_{X \mid \Lambda}(x \mid \lambda)=\frac{\lambda^{x} e^{-\lambda}}{x!}, x=0,1,2, \cdots
\]
Calculate \( E\left[e^{-\Lambda} \mid X=1\right] \).

\subsection*{Solution}

The marginal of \( X \) is given by
\begin{equation*}
    \implies
    f_{X}(x)
    =
    \int_{0}^{\infty} f_{X \mid \Lambda}(x \mid \lambda) f_{\Lambda}(\lambda) \, d\lambda
    =
    \int_{0}^{\infty} \frac{\lambda^{x} e^{-\lambda}}{x!} e^{-\lambda} \, d\lambda
    =
    \frac{1}{x!} \int_{0}^{\infty} \lambda^{x} e^{-2\lambda} \, d\lambda
\end{equation*}
We know that the Gamma function is given by
\begin{equation*}
    \Gamma(x)
    =
    \int_{0}^{\infty} t^{x-1} e^{-t} \, dt,
    \quad x>0
\end{equation*}
Using the change of variable \( t=2\lambda \), we have
\begin{align*}
    \implies
    f_{X}(x)
     & =
    \frac{1}{x!} \int_{0}^{\infty} {\left(\frac{t}{2}\right)}^{x} e^{-t} \frac{1}{2} \, dt
    =
    \frac{1}{x! \; 2^{x+1}} \int_{0}^{\infty} t^{x} e^{-t} \, dt
    =
    \frac{\Gamma(x+1)}{x! \; 2^{x+1}}
\end{align*}
We know that \( \Gamma(x+1)=x! \) for positive integers \( x \), so
\begin{equation}
    f_{X}(x)
    =
    \frac{1}{2^{x+1}},
    \quad
    x=0,1,2, \dots
\end{equation}
and \( f_{X}(x)=0 \) otherwise.
Now,
\vspace*{-1em}
\begin{align*}
    \implies
    f_{\Lambda \mid X}(\lambda \mid x)
     & =
    \frac{f_{X \mid \Lambda}(x \mid \lambda) f_{\Lambda}(\lambda)}{f_{X}(x)}
    =
    \frac{\cfrac{\lambda^{x} e^{-\lambda}}{x!} e^{-\lambda}}{\cfrac{1}{2^{x+1}}}
    =
    2^{x+1} \frac{\lambda^{x} e^{-2\lambda}}{x!}
    \\
    \implies
    f_{\Lambda \mid X}(\lambda \mid 1)
     & =
    2^{2} \frac{\lambda e^{-2\lambda}}{1!}
    =
    4 \lambda e^{-2\lambda}
\end{align*}
\begin{align*}
    \implies
    E\left[e^{-\Lambda} \mid X=1\right]
     & =
    \int_{0}^{\infty} e^{-\lambda} f_{\Lambda \mid X}(\lambda \mid 1) \, d\lambda
    =
    \int_{0}^{\infty} e^{-\lambda} 4 \lambda e^{-2\lambda} \, d\lambda
    =
    4 \int_{0}^{\infty} \lambda e^{-3\lambda} \, d\lambda
\end{align*}
Using the change of variable \( t=3\lambda \), we have
\begin{align*}
    \implies
    E\left[e^{-\Lambda} \mid X=1\right]
     & =
    4 \int_{0}^{\infty} \frac{t}{3} e^{-t} \frac{1}{3} \, dt
    =
    \frac{4}{9} \int_{0}^{\infty} t e^{-t} \, dt
    =
    \frac{4}{9} \Gamma(2)
    =
    \frac{4}{9} \cdot 1!
    =
    \boxed{
        \frac{4}{9}
    }
\end{align*}
