\section*{Question 2}

Let \( X, Y \) have joint density
\[
    f_{X Y}(x, y)=4 e^{-2 y}, 0<x<y
\]
Let \( Z=X+Y \).
Find \( E Z \).

\subsection*{Solution}

\begin{equation*}
    E[Z]
    =
    E[X+Y]
    =
    E[X] + E[Y]
\end{equation*}

\begin{align*}
    f_X (x)
     & =
    \int_{-\infty}^{\infty} f_{X Y}(x, y) \, dy
    =
    \int_{x}^{\infty} 4 e^{-2 y} \, dy
    =
    -2 e^{-2 y} \Big|_{x}^{\infty}
    =
    2 e^{-2 x}
    \\
    f_Y (y)
     & =
    \int_{-\infty}^{\infty} f_{X Y}(x, y) \, dx
    =
    \int_{0}^{y} 4 e^{-2 y} \, dx
    =
    4 e^{-2 y} x \Big|_{0}^{y}
    =
    4 y e^{-2 y}
\end{align*}

\begin{align*}
    \implies
    E[X]
     & =
    \int_{-\infty}^{\infty} x f_X(x) \, dx
    =
    \int_{0}^{\infty} 2 x e^{-2 x} \, dx
        =
        {\left[
                \cancel{2} x \frac{-1}{\cancel{2}} e^{-2 x}
                -
                \int \cancel{2} \frac{-1}{\cancel{2}} e^{-2 x} \, dx
                \right]}_{0}^{\infty}
    \\ & =
    {\left[
        -x e^{-2 x}
        -
        \frac{1}{2} e^{-2 x}
        \right]}_{0}^{\infty}
    =
    0 - 0 - \left( -0 - \frac{1}{2} \right)
    =
    \frac{1}{2}
    \\
    \implies
    E[Y]
     & =
    \int_{-\infty}^{\infty} y f_Y(y) \, dy
    =
    \int_{0}^{\infty} 4 y^2 e^{-2 y} \, dy
    =
    4 \int_{0}^{\infty} y^2 e^{-2 y} \, dy
    \\ & =
    4 \left(
    y^2 \frac{-1}{2} e^{-2 y} \Bigg|_{0}^{\infty}
    - \int_{0}^{\infty} 2y \frac{-1}{2} e^{-2 y} \, dy
    \right)
    =
    2 \int_{0}^{\infty} 2y e^{-2 y} \, dy
    =
    2 \frac{1}{2}
    =
    1
\end{align*}

\begin{equation*}
    \implies
    E[Z]
    =
    E[X] + E[Y]
    =
    \frac{1}{2} + 1
    =
    \frac{3}{2}
    \implies
    \boxed{
        E[Z] = \frac{3}{2}
    }
\end{equation*}
